theories/Handlers/Mailbox.v
@@ -1,0 +1,65 @@
+From Coq Require Import
+  Classes.EquivDec
+  SetoidClass
+  Classes.SetoidDec.
+
+Require Import
+  Queue
+  Multifunction
+  Pid
+  VM.
+
+From Hammer Require Import
+  Tactics.
+
+Section defn.
+  Context (AppMessage : Type).
+
+  Inductive Message :=
+  | appmsg : AppMessage -> Message.
+
+  Definition Mailbox := @Queue Message.
+
+  Let t := Pid.FMap.t Mailbox.
+
+  Inductive MBReq : Type :=
+  | send : Message -> PID -> MBReq.
+
+  Definition MBRet (req : MBReq) : Type :=
+    match req with
+    | send _ _ => True
+    end.
+
+  Definition do_send_msg (msg : Message) (to : PID) (mboxes : t) : t :=
+    match Pid.FMap.find to mboxes with
+    | Some mbox =>
+        Pid.FMap.add to (push msg mbox) mboxes
+    | None =>
+        mboxes
+    end.
+
+  Program Definition send_ (msg : Message) (to : PID) : MFunRet True t :=
+    {| morphism s x :=
+         x = (I, do_send_msg msg to s)
+    |}.
+  Next Obligation.
+    sauto.
+  Qed.
+
+  Definition mailbox_step (req : MBReq) : MFunRet (MBRet req) t :=
+    match req with
+    | send msg to => send_ msg to
+    end.
+
+  Check Pid.FMap.Equiv.
+
+  Let mailboxes_equiv := @Pid.FMap.Equiv Mailbox queue_equiv.
+
+  Instance mailboxHandler : @IOHandler MBReq MBRet :=
+    {|
+      h_state := t;
+      (* TODO: Use a setoid via mailboxes_equiv *)
+      h_setoid := eq_setoid _;
+      h_handler _ req := mailbox_step req
+    |}.
+End defn.
